ironfleet/ravana/RefinementProof.i.dfy
@@ -1,0 +1,39 @@
+include "Types.i.dfy"
+include "Refinement.i.dfy"
+include "Service.i.dfy"
+include "DistributedSystem.i.dfy"
+
+module Refinement_Proof_i {
+  import opened Types_i
+  import opened Refinement_i
+  import opened Service_i
+  import opened DistributedSystem_i
+
+  /** MAIN LEMMA **/
+
+  /*
+  lemma rs_refines_ss(rs: RState, rs': RState)
+  requires rstate_valid(rs)
+  requires RS_Next(rs, rs')
+  ensures rstate_valid(rs')
+  ensures Service_Next(refinement(rs), refinement(rs'))
+  {
+  }
+  */
+
+  lemma lemma_refines_Logger_InitNewMaster(rs: RState, rs': RState)
+  requires rstate_valid(rs)
+
+  requires LEnvironment_Next(rs.environment, rs'.environment)
+  requires rs.environment.nextStep.LEnvStepHostIos?
+  requires rs.endpoint_logger == rs'.endpoint_logger
+  requires rs.environment.nextStep.actor == rs'.endpoint_logger
+  requires NodeNext_Logger(rs.server_logger, rs'.server_logger, rs.environment.nextStep.ios)
+  requires rs.server_controllers == rs'.server_controllers
+  requires rs.server_switches == rs'.server_switches
+
+  ensures rstate_valid(rs')
+  ensures refinement(rs) == refinement(rs')
+  {
+  }
+}
